% func-image.tex

%%%%%%%%%%%%%%%
\begin{frame}{}
  \begin{definition}[Restriction]
    The {\it restriction} of a function $f$ to $X$ is the \purple{function}:

    \[
      f|_{X} = \set{(x, y) \in f \mid x \in X}
    \]
  \end{definition}

  \[
    f: A \to B
  \]

  \pause
  \[
    f|_{X}: A \cap X \to B
  \]
  \[
    f|_{X}(x) = f(x), \forall x \in A \cap X
  \]
\end{frame}
%%%%%%%%%%%%%%%

%%%%%%%%%%%%%%%
\begin{frame}{}
  \begin{definition}[Image]
    The {\it image} of $X$ under a function $f$ is the \teal{set}
    \[
      {f(X) = \set{\purple{b \in \text{ran}(f)} \mid \exists a \in X: (a, b) \in f}}
    \]
  \end{definition}

  \vspace{0.50cm}
  \begin{definition}[Inverse Image]
    The {\it inverse image} of $Y$ under a function $f$ is the \teal{set}
    \[
      {f^{-1}(Y) = \set{\purple{a \in \text{dom}(f)} \mid \exists b \in Y: (a, b) \in f}}
    \]
  \end{definition}

  \pause
  \[
    \textcolor{gray}{X \subseteq \dom{f},\; Y \subseteq \ran{f}} \text{ are not necessary}
  \]

  \pause
  \[
    f \text{ may not be \red{invertible} in } f^{-1}(Y)
  \]
\end{frame}
%%%%%%%%%%%%%%%

%%%%%%%%%%%%%%%
\begin{frame}{}
  \[
    \red{\boxed{y \in f(X) \iff \exists x \in \dom{f} \land X: y = f(x)}}
  \]

  \vspace{0.60cm}
  \[
    \red{\boxed{x \in f^{-1}(Y) \iff f(x) \in Y}}
  \]
\end{frame}
%%%%%%%%%%%%%%%

%%%%%%%%%%%%%%%
\begin{frame}{}
  \begin{theorem}[Properties of $f$ and $f^{-1}$ (UD Theorem $17.7$)]
    \[
      f: A \to B \qquad \textcolor{gray}{A_1, A_2 \subseteq A,\; B_1, B_2 \subseteq B}
    \]

    \vspace{-0.10cm}
    \begin{enumerate}[(i)]
      \setlength{\itemsep}{10pt}
      \item \purple{$f$ preserves only $\subseteq$ and $\cup$:}
	\begin{enumerate}[(1)]
	  \setlength{\itemsep}{4pt}
	  \item $A_1 \subseteq A_2 \implies f(A_1) \subseteq f(A_2)$
	  \item $f(A_1 \cup A_2) = f(A_1) \cup f(A_2)$
	  \item $f(A_1 \cap A_2) \subseteq f(A_1) \cap f(A_2)$
	  \item $f(A_1 \setminus A_2) \subseteq f(A_1) \setminus f(A_2)$
	\end{enumerate}
      \item \purple{$f^{-1}$ preserves $\subseteq, \cup, \cap,$ and $\setminus$:}
	\begin{enumerate}[(1)]
	  \setlength{\itemsep}{4pt}
	  \setcounter{enumii}{4}
	  \item $B_1 \subseteq B_2 \implies f^{-1}(B_1) \subseteq f^{-1}(B_2)$
	  \item $f^{-1}(B_1 \cup B_2) = f^{-1}(B_1) \cup f^{-1}(B_2)$
	  \item $f^{-1}(B_1 \cap B_2) = f^{-1}(B_1) \cap f^{-1}(B_2)$
	  \item $f^{-1}(B_1 \setminus B_2) = f^{-1}(B_1) \setminus f^{-1}(B_2)$
	\end{enumerate}
    \end{enumerate}
  \end{theorem}
\end{frame}
%%%%%%%%%%%%%%%

%%%%%%%%%%%%%%%
\begin{frame}{}
  \begin{theorem}[UD Problem 17.5]
    \[
      f: A \to B
    \]

    \[
      f(A_1 \cap A_2) \red{\;\subseteq\;} f(A_1) \cap f(A_2)
    \]
  \end{theorem}

  \pause
  \vspace{0.60cm}
  \begin{center}
    \red{$Q:$ When does $f(A_1 \cap A_2) \red{\;=\;} f(A_1) \cap f(A_2)$ hold?} \pause\\[10pt]
    \teal{$f$ is injective.}
  \end{center}
\end{frame}
%%%%%%%%%%%%%%%

%%%%%%%%%%%%%%%
\begin{frame}{}
  \begin{theorem}[Properties of $f$ and $f^{-1}$ (UD Theorem $17.7$)]
    \[
      f: A \to B
    \]

    \vspace{-0.10cm}
    \begin{enumerate}[(i)]
      \setcounter{enumi}{2}
      \item $f$ and $f^{-1}$: \\[8pt]
	\begin{enumerate}[(1)]
	  \setlength{\itemsep}{10pt}
	  \setcounter{enumii}{8}
	    \item $\teal{A_0 \subseteq A} \implies A_0 \subseteq f^{-1}(f(A_0))$
	    \item $B_0 \supseteq f(f^{-1}(B_0))$
	\end{enumerate}
    \end{enumerate}
  \end{theorem}
\end{frame}
%%%%%%%%%%%%%%%

%%%%%%%%%%%%%%%
\begin{frame}{}
  \[
    f: A \to B
  \]

  \begin{theorem}[UD Problem 17.8]
    \[
      A_0 \subseteq A \implies A_0 \subseteq f^{-1}(f(A_0))
    \]
  \end{theorem}

  \pause
  \vspace{0.30cm}
  \begin{theorem}[]
    \[
      B_0 \supseteq f(f^{-1}(B_0))
    \]
  \end{theorem}

  \pause
  \vspace{0.30cm}
  \begin{center}
    \red{$Q$: When does $B_0 = f(f^{-1}(B_0))$ hold?} \pause \\[10pt]

    \teal{$f$ is surjective and $B_0 \subseteq B$.} \pause \\[5pt]
    \teal{$B_0 \subseteq \ran{f}$}
  \end{center}
\end{frame}
%%%%%%%%%%%%%%%
